[[Действие группы на множестве]]
[[Стабилизатор подмножества]]
[[Сопряжение группы]]
#### Формулировка
Пусть $a \in G, N \subset M$. Тогда $St(aN) = I_{a^{-1}}(St(N))$. 

>[!info]+ Смысл
>Используя $I_{a^{-1}}$ мы "распаковываем" элементы из $St(N)$ и домножаем слева на $a$. 
#### Доказательство
$$
\begin{align}
	x \in St(aN) \iff \\
	(xa)N = x(aN) = aN \iff \\
	a^{-1}((xa)N) = a^{-1}(aN) \iff \\
	I_a(x)N = (a^{-1}xa)N = (a^{-1}a)N = eN = N \iff\\
	I_a(x) \in St(N) \\
	\\
	St(aN) = \{x \in G : x(aN) = aN\} \\
	St(N) = \{I_a(x) : x\in G : I_a(x)N = N\}\\
	I_{a^{-1}}(St(N)) = \{x : x \in G : a^{-1}xaN = N\} =\\
	= \{x : x \in G : x(aN) = aN\} = \{x \in G : x(aN) = aN\} = St(aN)\\
	\\
	St(aN) = I_{a^{-1}}(St(N))
\end{align}
$$





